theories/Implication.v
@@ -1,0 +1,190 @@
+Require Import Heapster.Permissions.
+
+
+Section implication.
+  Inductive type :=
+  | TUnit : type
+  | TNat : type
+  .
+
+  Inductive term (T : Type) :=
+  | Var : T -> term T
+  .
+
+  Context (T : Type).
+
+  Definition apply {T} (P : T -> Perms) (x : T) := P x.
+  Notation "x : P" := (apply P x) (at level 40).
+
+  Definition empty := bottom_Perms.
+  Definition true_p := fun (_ : T) => bottom_Perms.
+
+  Lemma drop (x : T) P : x:P ⊦ empty.
+  Proof.
+    repeat intro. simpl. auto.
+  Qed.
+  Lemma true_intro (x : T) : empty ⊦ x:true_p.
+  Proof.
+    repeat intro; auto.
+  Qed.
+
+  (* Perms where domain is x = y *)
+  Program Definition eq_p (y : T) :=
+    fun (x : T) =>
+      {|
+        in_Perms := fun _ => x = y;
+      |}.
+
+  Lemma eq_refl (x : T) : empty ⊦ x:eq_p(x).
+  Proof.
+    repeat intro. simpl. auto.
+  Qed.
+
+  Lemma eq_trans (x y z : T) : x:eq_p(y) ** y:eq_p(z) ⊦ x:eq_p(z).
+  Proof.
+    repeat intro. destruct H as [p1 [p2 [Hp1 [Hp2 ?]]]]. simpl in *. subst. auto.
+  Qed.
+
+  Lemma eq_elim (x y : T) P : x:eq_p(y) ** y:P ⊦ x:P.
+  Proof.
+    repeat intro. destruct H as [p1 [p2 [Hp1 [Hp2 ?]]]].
+    destruct Hp1.
+    eapply Perms_upwards_closed; eauto. etransitivity. apply lte_r_sep_conj_perm. eauto.
+  Qed.
+
+  Lemma copy (x : T) P : (forall p, p ∈ x:P -> read_perm p) ->
+                    x:P ⊦ x:P ** x:P.
+  Proof.
+    repeat intro. exists p, p. split; [| split]; auto.
+    specialize (H _ H0). apply separate_self_read in H. split; intros; simpl; eauto.
+    induction H1.
+    - destruct H1; auto.
+    - etransitivity; eauto.
+  Qed.
+
+  Lemma or_left_intro (x : T) P Q : x:P ⊦ meet_Perms2 (x:P) (x:Q).
+  Proof.
+    repeat intro. exists (x:P). split; auto.
+  Qed.
+  Lemma or_right_intro (x : T) P Q : x:Q ⊦ meet_Perms2 (x:P) (x:Q).
+  Proof.
+    repeat intro. exists (x:Q). split; auto.
+  Qed.
+
+  Lemma or_elim (x : T) P Q R : x:P ⊦ R ->
+                                x:Q ⊦ R ->
+                                meet_Perms2 (x:P) (x:Q) ⊦ R.
+  Proof.
+    repeat intro. destruct H1 as [X [? ?]]. destruct H1; subst; auto.
+  Qed.
+
+  Definition exists_Perms T (P : T -> T -> Perms) : T -> Perms :=
+    fun x => meet_Perms (fun Q => exists y, Q = x:P(y)).
+
+  Lemma exists_intro (x y : T) P : x:P(y) ⊦ x:(exists_Perms T P).
+  Proof.
+    repeat intro. exists (x:P(y)). split; auto. exists y; auto.
+  Qed.
+
+  Lemma exists_elim (x : T) P R : (forall (y': T), x:P(y') ⊦ R) ->
+                                  x:(exists_Perms T P) ⊦ R.
+  Proof.
+    repeat intro. destruct H0 as [X [[? ?] ?]]. subst. eapply H; eauto.
+  Qed.
+
+  Class Ilookup (x : T) (lhs : Perms) (x_P : T -> Perms) rem : Prop :=
+    ilookup : lhs ⊦ x:x_P ** rem.
+
+  Instance Ilookup_empty x :
+    Ilookup x empty true_p empty.
+  Proof.
+    red. rewrite sep_conj_Perms_bottom_identity. reflexivity.
+  Qed.
+
+  Instance Ilookup_base x P lhs :
+    Ilookup x (x:P ** lhs) P lhs.
+  Proof.
+    red. reflexivity.
+  Qed.
+
+  Instance Ilookup_step (T' : Type) (x: T) (x' : T') lhs P P' rem :
+    Ilookup x lhs P rem ->
+    Ilookup x (x':P' ** lhs) P (x':P' ** rem).
+  Proof.
+    intros. red. red in H.
+    Check Proper_entails_Perms_entails_Perms.
+    rewrite (sep_conj_Perms_commut (x:P) _). rewrite <- sep_conj_Perms_assoc.
+    apply sep_conj_Perms_monotone; intuition. rewrite sep_conj_Perms_commut. apply H.
+  Qed.
+
+  Class Ivar (x : T) P_lhs lhs P_rhs rem : Prop :=
+    ivar : x:P_lhs ** lhs ⊦ x:P_rhs ** rem.
+
+  Class Implies (lhs rhs rem : Perms) : Prop :=
+    impl: lhs ⊦ rhs ** rem.
+
+  Instance Implies_empty lhs :
+    Implies lhs empty lhs.
+  Proof.
+    red. rewrite sep_conj_Perms_bottom_identity. reflexivity.
+  Qed.
+
+  Instance Implies_nonempty x lhs rhs P_lhs P_rhs rem1 rem2 rem3 :
+    Ilookup x lhs P_lhs rem1 ->
+    Ivar x P_lhs rem1 P_rhs rem2 ->
+    Implies rem2 rhs rem3 ->
+    Implies lhs (x:P_rhs ** rhs) rem3.
+  Proof.
+    intros. red. red in H, H0, H1. etransitivity. apply H.
+    etransitivity. apply H0. rewrite <- sep_conj_Perms_assoc.
+    apply sep_conj_Perms_monotone; intuition.
+  Qed.
+
+  Instance Ivar_true x lhs P_lhs :
+    Ivar x P_lhs lhs true_p (x:P_lhs ** lhs).
+  Proof.
+    red. rewrite (sep_conj_Perms_commut (x:true_p) _).
+    rewrite <- sep_conj_Perms_bottom_identity at 1. rewrite sep_conj_Perms_commut.
+    apply sep_conj_Perms_monotone; reflexivity.
+  Qed.
+
+  Instance Ivar_eq_refl x lhs P_lhs :
+    Ivar x P_lhs lhs (eq_p(x)) (x:P_lhs ** lhs).
+  Proof.
+    red. rewrite (sep_conj_Perms_commut (x:eq_p(x))).
+    rewrite <- sep_conj_Perms_bottom_identity at 1. rewrite sep_conj_Perms_commut.
+    apply sep_conj_Perms_monotone; intuition.
+    (* typeclasses eauto. should work ? *)
+    etransitivity. apply eq_refl.
+    reflexivity.
+  Qed.
+
+  Instance Ivar_eq_elim x y lhs P_y P_x rem1 rem2:
+    Ilookup y lhs P_y rem1 ->
+    Ivar x P_y rem1 P_x rem2 ->
+    Ivar x (eq_p(y)) lhs P_x rem2.
+  Proof.
+    intros. red in H, H0. red. etransitivity. 2: { apply H0. }
+    repeat intro. destruct H1 as [? [? [? [? ?]]]]. destruct H1. apply H.
+    eapply Perms_upwards_closed. eauto. etransitivity. apply lte_r_sep_conj_perm. eauto.
+    (* todo use eq_elim lemma *)
+  Qed.
+
+  (* Typeclasses eauto := debug. *)
+
+  Goal forall x y, Ilookup x (x:true_p ** (y:true_p ** empty)) true_p (y:true_p ** empty).
+  Proof.
+    typeclasses eauto.
+  Qed.
+
+  Goal forall x, Implies empty (x:true_p ** empty) (x:true_p ** empty).
+  Proof.
+    typeclasses eauto.
+  Qed.
+
+  Goal forall x y, Implies empty (x:true_p ** (y:true_p ** empty)) (x:true_p ** (y:true_p ** empty)).
+  Proof.
+    typeclasses eauto.
+  Qed.
+
+End implication.
