theories/Typing.v
@@ -1,0 +1,352 @@
+Require Import Heapster.Permissions.
+
+From Coq Require Import
+     Classes.Morphisms
+     Classes.RelationClasses
+     Relations.Relation_Operators
+     Relations.Operators_Properties.
+
+From ITree Require Import
+     ITree
+     ITreeFacts
+     Events.State
+     Events.Nondeterminism
+     Eq.Eq
+     Eq.UpToTaus.
+
+From Paco Require Import
+     paco.
+
+Import ITreeNotations.
+Import ITree.Basics.Basics.Monads.
+
+Require Import ITree.Eq.EqAxiom.
+
+Section ts.
+
+  Definition E := (stateE config +' nondetE).
+
+  Context {R : Type}.
+
+  Definition par_match
+             (par : itree E R -> itree E R -> itree E R)
+             (t1 t2 : itree E R)
+    : itree E R :=
+    vis Or (fun b : bool =>
+              if b then
+                match (observe t1) with
+                | RetF _ => t2
+                | TauF t => Tau (par t t2)
+                | VisF o k => vis o (fun x => par (k x) t2)
+                end
+              else
+                match (observe t2) with
+                | RetF _ => t1
+                | TauF t => Tau (par t1 t)
+                | VisF o k => vis o (fun x => par t1 (k x))
+                end).
+
+  CoFixpoint par (t1 t2 : itree E R) := par_match par t1 t2.
+
+  Lemma rewrite_par : forall t1 t2, par t1 t2 = par_match par t1 t2.
+  Proof.
+    intros. apply bisimulation_is_eq. revert t1 t2.
+    ginit. gcofix CIH. intros. gstep. unfold par. constructor. red. intros.
+    apply Reflexive_eqit_gen_eq. (* not sure why reflexivity doesn't work here *)
+  Qed.
+
+  Variant step : itree E R -> config -> itree E R -> config -> Prop :=
+  | step_tau : forall t c, step (Tau t) c t c
+  | step_nondet_true : forall k c, step (vis Or k) c (k true) c
+  | step_nondet_false : forall k c, step (vis Or k) c (k false) c
+  | step_get : forall k c, step (vis (Get _) k) c (k c) c
+  | step_put : forall k c c', step (vis (Put _ c') k) c (k tt) c'
+  .
+
+  Lemma step_bind : forall (t1 t2 : itree E R) (c1 c2 : config) (k : R -> itree E R),
+      step t1 c1 t2 c2 ->
+      step (t1 >>= k) c1 (t2 >>= k) c2.
+  Proof.
+    intros. inversion H; subst.
+    - pose proof (bind_tau _ t2 k) as bind_tau.
+      apply bisimulation_is_eq in bind_tau. rewrite bind_tau. constructor.
+    - pose proof (bind_vis _ _ (subevent _ Or) k0 k) as bind_vis.
+      apply bisimulation_is_eq in bind_vis. rewrite bind_vis. constructor.
+    - pose proof (bind_vis _ _ (subevent _ Or) k0 k) as bind_vis.
+      apply bisimulation_is_eq in bind_vis. rewrite bind_vis. constructor.
+    - pose proof (bind_vis _ _ (subevent _ (Get _)) k0 k) as bind_vis.
+      apply bisimulation_is_eq in bind_vis. rewrite bind_vis. constructor.
+    - pose proof (bind_vis _ _ (subevent _ (Put _ c2)) k0 k) as bind_vis.
+      apply bisimulation_is_eq in bind_vis. rewrite bind_vis. constructor.
+  Qed.
+
+  Lemma step_ret_bind : forall (t1 t2 : itree E R) (c1 c2 : config) (r : R),
+      step t1 c1 t2 c2 ->
+      step (Ret r;; t1) c1 t2 c2.
+  Proof.
+    intros. pose proof (bind_ret_l r (fun _ => t1)) as bind_ret.
+    apply bisimulation_is_eq in bind_ret. rewrite bind_ret. assumption.
+  Qed.
+
+  (* to handle the nondeterminism, par needs double the amount of steps *)
+  Lemma par_step_left : forall (t1 t2 t' : itree E R) (c c' : config),
+      step t1 c t2 c' ->
+      exists t'', step (par t1 t') c t'' c /\ step t'' c (par t2 t') c'.
+  Proof.
+    inversion 1; subst;
+      (rewrite rewrite_par; unfold par_match; simpl; repeat eexists; constructor).
+  Qed.
+  Lemma par_step_right : forall (t1 t2 t' : itree E R) (c c' : config),
+      step t1 c t2 c' ->
+      exists t'', step (par t' t1) c t'' c /\ step t'' c (par t' t2) c'.
+  Proof.
+    inversion 1; subst;
+      (rewrite rewrite_par; unfold par_match; simpl; repeat eexists; constructor).
+  Qed.
+
+  Definition sep_step p q : Prop :=
+    (* (forall x, dom p x -> dom q x) /\ *)
+    (forall r, p ⊥ r -> q ⊥ r).
+
+  Instance sep_step_refl : Reflexive sep_step.
+  Proof.
+    repeat intro; auto.
+  Qed.
+
+  Instance sep_step_trans : Transitive sep_step.
+  Proof.
+    repeat intro. auto.
+  Qed.
+
+  Lemma sep_step_lte : forall p p' q, p <= p' -> sep_step p q -> sep_step p' q.
+  Proof.
+    repeat intro. apply H0. symmetry. symmetry in H1. eapply separate_antimonotone; eauto.
+  Qed.
+
+  Lemma sep_step_view : forall p q x y, sep_step p q -> view p x y -> view q x y.
+  Proof.
+    intros. specialize (H (sym_upd_perm p) (separate_self_sym _)).
+    apply H; auto.
+  Qed.
+
+  Lemma sep_step_upd : forall p q x y, sep_step p q ->
+                                  upd q x y ->
+                                  clos_refl_sym_trans config (upd p) x y.
+  Proof.
+    intros. specialize (H (sym_upd_perm p) (separate_self_sym _)).
+    apply H; auto.
+  Qed.
+
+  Lemma sep_step_sep_conj_l : forall p1 p2 q, p1 ⊥ q -> sep_step p1 p2 -> sep_step (p1 * q) (p2 * q).
+  Proof.
+    intros p1 p2 q ? ?.
+    repeat intro; auto. symmetry in H1. symmetry. apply separate_sep_conj_perm; symmetry; auto.
+    - apply H0. symmetry. eapply separate_sep_conj_perm_l; eauto.
+    - symmetry. eapply separate_sep_conj_perm_r; eauto.
+  Qed.
+  Lemma sep_step_sep_conj_r : forall p1 p2 q, p1 ⊥ q -> sep_step p1 p2 -> sep_step (q * p1) (q * p2).
+  Proof.
+    intros p1 p2 q ? ?.
+    repeat intro; auto. symmetry in H1. symmetry. apply separate_sep_conj_perm; symmetry; auto.
+    - symmetry. eapply separate_sep_conj_perm_l; eauto.
+    - apply H0. symmetry. eapply separate_sep_conj_perm_r; eauto.
+    - symmetry. auto.
+  Qed.
+
+  Variant typing_perm_gen typing (p : perm) (t : itree E R) : Prop :=
+  | cond : (forall c, dom p c ->
+                 forall t' c',
+                   step t c t' c' ->
+                   (
+                     (* we step to configs that satisfy the perm *)
+                     (upd p c c') /\
+                     (* we step to machines that are well-typed by some other perm that maintains separation *)
+                     (exists p', typing p' t' /\ sep_step p p' /\ dom p' c'))) ->
+           typing_perm_gen typing p t.
+
+  Definition typing_perm p t := paco2 typing_perm_gen bot2 p t.
+
+  Lemma typing_perm_gen_mon : monotone2 typing_perm_gen.
+  Proof.
+    repeat intro.
+    inversion IN. econstructor. intros. specialize (H _ H0 _ _ H1).
+    destruct H as [? [? [? ?]]]. split; eauto.
+  Qed.
+  Hint Resolve typing_perm_gen_mon : paco.
+
+  Lemma rewrite_spin : (ITree.spin : itree E R) = Tau (ITree.spin).
+  Proof.
+    intros. apply bisimulation_is_eq.
+    ginit. gcofix CIH. gstep. unfold ITree.spin. constructor.
+    apply Reflexive_eqit_gen_eq.
+  Qed.
+
+  Lemma typing_perm_lte : forall p q t, typing_perm p t -> p <= q -> typing_perm q t.
+  Proof.
+    intros. pcofix CIH. pstep. constructor; intros.
+    pinversion H. edestruct H3; eauto. split; eauto.
+    destruct H5 as [p' [? [? ?]]]. exists p'. split; [| split]; auto.
+    - pclearbot. left. eapply paco2_mon_bot; eauto.
+    - eapply sep_step_lte; eauto.
+  Qed.
+
+  Definition typing P t := forall p, p ∈ P -> typing_perm p t.
+
+  Lemma type_lte : forall P Q t, typing P t -> P ⊑ Q -> typing Q t.
+  Proof.
+    repeat intro. specialize (H p (H0 _ H1)). auto.
+  Qed.
+
+  Lemma type_spin : forall P, typing P ITree.spin.
+  Proof.
+    pcofix CIH. intros. pstep. constructor. intros. rewrite rewrite_spin in H1.
+    inversion H1; subst. split; try reflexivity.
+    exists p. split; eauto; intuition.
+  Qed.
+
+  Lemma type_ret : forall P r, typing P (Ret r).
+  Proof.
+    repeat intro.
+    pstep. constructor. intros. inversion H1.
+  Qed.
+
+  Lemma type_top : forall t, typing top_Perms t.
+  Proof.
+    repeat intro. pstep. constructor. intros. inversion H.
+  Qed.
+
+  Lemma type_tau : forall P t, typing P t -> typing P (Tau t).
+  Proof.
+    repeat intro. specialize (H _ H0). pinversion H.
+    pfold. econstructor. intros.
+    inversion H3; subst.
+    split; intuition.
+    exists p. split; intuition.
+  Qed.
+
+  Lemma frame : forall P1 P2 t, typing P1 t -> typing (P1 ** P2) t.
+  Proof.
+    intros. eapply type_lte; eauto. apply lte_l_sep_conj_Perms.
+  Qed.
+  (* todo get proper instance working *)
+  Lemma frame' : forall P1 P2 t, typing P2 t -> typing (P1 ** P2) t.
+  Proof.
+    intros. eapply type_lte; eauto. apply lte_r_sep_conj_Perms.
+  Qed.
+
+  Require Import Coq.Program.Equality.
+
+  Lemma parallel_perm : forall p1 p2 t1 t2,
+      typing_perm p1 t1 -> typing_perm p2 t2 -> typing_perm (p1 * p2) (par t1 t2).
+  Proof.
+    pcofix CIH. intros p1 p2 t1 t2 Ht1 Ht2.
+    pstep. econstructor. intros c [Hdom1 [Hdom2 Hsep]] t' c' Hstep.
+    rewrite rewrite_par in Hstep. unfold par_match in Hstep.
+    dependent destruction Hstep; split; try reflexivity.
+    { destruct (observe t1) eqn:?.
+      - exists p2. split; [left; eapply paco2_mon_bot; eauto | split]; auto.
+        repeat intro. symmetry. symmetry in H. eapply separate_sep_conj_perm_r; eauto.
+      - symmetry in Heqi. pose proof (bisimulation_is_eq _ _ (simpobs Heqi)) as Heqi'.
+        rewrite Heqi' in Ht1.
+        pinversion Ht1. destruct (H _ Hdom1 _ _ (step_tau _ _)) as [? [p [? [? ?]]]].
+        exists (p * p2). pclearbot. split; [| split].
+        + left. pstep. constructor. intros. inversion H5; subst.
+          split; intuition. exists (p * p2). split; [| split]; intuition.
+        + apply sep_step_sep_conj_l; auto.
+        + split; [| split]; auto.
+      - symmetry in Heqi. pose proof (bisimulation_is_eq _ _ (simpobs Heqi)) as Heqi'.
+        rewrite Heqi' in Ht1.
+        destruct e; [destruct s | destruct n]; pinversion Ht1; exists (p1 * p2);
+          (split; intuition; [| split; [| split]]; auto);
+          left; pstep; constructor; intros ? [Hdom1' [Hdom2' Hsep']] ? ? Hstep;
+            inversion Hstep; auto_inj_pair2; subst.
+        + destruct (H _ Hdom1' _ _ (step_get _ _)) as [? [p [? [? ?]]]]. pclearbot.
+          split; intuition.
+          exists (p * p2). split; [| split]; auto.
+          * apply sep_step_sep_conj_l; auto.
+          * split; [| split]; auto.
+        + destruct (H _ Hdom1' _ _ (step_put _ _ _)) as [? [p [? [? ?]]]]. pclearbot.
+          split; [constructor |]; auto.
+          exists (p * p2). split; [| split]; auto.
+          * apply sep_step_sep_conj_l; auto.
+          * split; [| split]; auto.
+            rewrite dom_respects. 2: { symmetry. apply Hsep'. apply H0. } auto.
+        + destruct (H _ Hdom1' _ _ (step_nondet_true _ _)) as [? [p [? [? ?]]]]. pclearbot.
+          split; intuition.
+          exists (p * p2). split; [| split]; auto.
+          * apply sep_step_sep_conj_l; auto.
+          * split; [| split]; auto.
+        + destruct (H _ Hdom1' _ _ (step_nondet_false _ _)) as [? [p [? [? ?]]]]. pclearbot.
+          split; intuition.
+          exists (p * p2). split; [| split]; auto.
+          * apply sep_step_sep_conj_l; auto.
+          * split; [| split]; auto.
+    }
+    { symmetry in Hsep. destruct (observe t2) eqn:?.
+      - exists p1. split; [left; eapply paco2_mon_bot; eauto | split]; auto.
+        repeat intro. symmetry. symmetry in H. eapply separate_sep_conj_perm_l; eauto.
+      - symmetry in Heqi. pose proof (bisimulation_is_eq _ _ (simpobs Heqi)) as Heqi'.
+        rewrite Heqi' in Ht2.
+        pinversion Ht2. destruct (H _ Hdom2 _ _ (step_tau _ _)) as [? [p [? [? ?]]]].
+        exists (p1 * p). pclearbot. split; [| split].
+        + left. pstep. constructor. intros. inversion H5; subst.
+          split; intuition. exists (p1 * p). split; [| split]; intuition.
+        + apply sep_step_sep_conj_r; auto.
+        + split; [| split]; auto. symmetry. apply H2; auto.
+      - symmetry in Heqi. pose proof (bisimulation_is_eq _ _ (simpobs Heqi)) as Heqi'.
+        rewrite Heqi' in Ht2. symmetry in Hsep.
+        destruct e; [destruct s | destruct n]; pinversion Ht2; exists (p1 * p2);
+          (split; intuition; [| split; [| split]]; auto);
+          left; pstep; constructor; intros ? [Hdom1' [Hdom2' Hsep']] ? ? Hstep;
+            inversion Hstep; auto_inj_pair2; subst; symmetry in Hsep.
+        + destruct (H _ Hdom2' _ _ (step_get _ _)) as [? [p [? [? ?]]]]. pclearbot.
+          split; intuition.
+          exists (p1 * p). split; [| split]; auto.
+          * apply sep_step_sep_conj_r; auto.
+          * split; [| split]; auto. symmetry. apply H2; auto.
+        + destruct (H _ Hdom2' _ _ (step_put _ _ _)) as [? [p [? [? ?]]]]. pclearbot.
+          split; [constructor |]; auto.
+          exists (p1 * p). split; [| split]; auto.
+          * apply sep_step_sep_conj_r; auto.
+          * split; [| split]; auto. 2: symmetry; apply H2; auto.
+            rewrite dom_respects. 2: { symmetry. apply Hsep'. apply H0. } auto.
+        + destruct (H _ Hdom2' _ _ (step_nondet_true _ _)) as [? [p [? [? ?]]]]. pclearbot.
+          split; intuition.
+          exists (p1 * p). split; [| split]; auto.
+          * apply sep_step_sep_conj_r; auto.
+          * split; [| split]; auto. symmetry. apply H2; auto.
+        + destruct (H _ Hdom2' _ _ (step_nondet_false _ _)) as [? [p [? [? ?]]]]. pclearbot.
+          split; intuition.
+          exists (p1 * p). split; [| split]; auto.
+          * apply sep_step_sep_conj_r; auto.
+          * split; [| split]; auto. symmetry. apply H2; auto.
+      }
+  Qed.
+
+  Lemma parallel : forall P1 P2 t1 t2,
+      typing P1 t1 -> typing P2 t2 -> typing (P1 ** P2) (par t1 t2).
+  Proof.
+    intros P1 P2 t1 t2 Ht1 Ht2 p [p1 [p2 [? [? ?]]]].
+    assert (Hp1: p ∈ P1).
+    { eapply Perms_upwards_closed; eauto. etransitivity; eauto. apply lte_l_sep_conj_perm. }
+    assert (Hp2: p ∈ P2).
+    { eapply Perms_upwards_closed; eauto. etransitivity; eauto. apply lte_r_sep_conj_perm. }
+    specialize (Ht1 _ H).
+    specialize (Ht2 _ H0). eapply typing_perm_lte; eauto. eapply parallel_perm; eauto.
+  Qed.
+End ts.
+
+Import ITreeNotations.
+Import ITree.Basics.Basics.Monads.
+
+Definition test : itree (stateE config +' _) unit :=
+  par
+    (x <- (trigger (Get _)) ;; (trigger (Put _ x)))
+    (par (vis (Get _) (fun x => Ret tt))
+         (Ret tt)).
+
+(* Compute (burn 10 test). *)
+
+(* Eval cbv in (burn 10 (step (trigger (Put _ 0)) 1)). *)
+(* Eval cbn in (burn 10 (step test 1)). *)
+(* Eval cbn in (burn 10 (run_state test 1)). *)
